alias:: 反证法

- [[proof by contraposition]] make use of the fact that the conditional statement $p → q$ is equivalent to its contrapositive, $¬q → ¬p$. This means that the conditional statement $p → q$ can be proved by showing that its [[contrapositive]], $¬q → ¬p$, is true. In a proof by contraposition of $p → q$, we take $¬q$ as a [[premise]], and using [[axioms]], definitions, and previously proven [[theorems]], together with [[rules of inference]], we show that $¬p$ must follow.
- $$(\neg p\Rightarrow\neg q)\Longleftrightarrow (p\Rightarrow q)$$
-